Wavelet/Simulation.lean
@@ -9,6 +9,7 @@ import Wavelet.Simulation.Ret
 import Wavelet.Simulation.Tail
 import Wavelet.Simulation.Op
 import Wavelet.Simulation.Br
+import Wavelet.Simulation.Call
 
 namespace Wavelet.Simulation
 
